

Rotunno (1983) Problem

Now consider $Q = e^{-z} e^{\sigma t} \frac{1}{\pi} \left(\frac{\pi}{2} + \tan^{-1} \frac{x}{L} \right)$.

The idea here is that we will now transition smoothly from the "sea" region (no heating) to the "land" region (heating) over a "coastal zone". The width of the coastal zone is governed by L . We recover the Heaviside problem as $L \rightarrow 0$. Note

$$\tilde{Q} = e^{-z} 2\pi \delta(\sigma-1) \frac{1}{\pi} \left(\frac{\pi}{2} + \tan^{-1} \frac{x}{L} \right),$$

$$\frac{\partial \tilde{Q}}{\partial x} = e^{-z} 2\pi \delta(\sigma-1) \frac{1}{\pi} \left(\frac{1}{(\frac{x}{L})^2 + 1} \right) \cdot \frac{1}{L}$$

$$\widehat{\frac{\partial Q}{\partial x}} = e^{-z} 2\pi \delta(\sigma-1) e^{-L|k|}.$$

So the only change from the Heaviside problem is the factor $e^{-L|k|}$. So (22)

from the Heaviside problem is now

$$\psi = \frac{-8(0-1)}{B^2 2i} \left\{ \int_0^\infty \left(\frac{-1}{(h/A+i)} + \frac{1}{(h/A-i)} \right) \left(e^{i h/A z} - e^{-z} \right) e^{i h x - L h} dh \right. \\ \left. + \int_{-\infty}^0 \left(\frac{-1}{(h/A+i)} + \frac{1}{(h/A-i)} \right) \left(e^{-i h/A z} - e^{-z} \right) e^{i h x - L h} dh \right\},$$

recalling we choose $\frac{1}{A}$ so that $\chi(1/A) > 0$.

So define

$$L_1 = \frac{1}{A} z + x + iL, \quad L_2 = -\frac{1}{A} z + x - iL,$$

$$\text{Note } \operatorname{Im}(L_1) = \operatorname{Im}\left(\frac{1}{A} z + x + iL\right)$$

$$= \left(\operatorname{Im}\left(\frac{1}{A}\right) + L \right) \operatorname{sgn}(z) > 0, \quad \text{noting } z \geq 0$$

and $L > 0$. Also, note $\arg(-iL_1)$

$$= \operatorname{atan2}(\operatorname{Im}(-iL_1), \operatorname{Re}(-iL_1))$$

$$= \operatorname{atan2}(-\operatorname{Re}\left(\frac{1}{A}\right)z - x, \operatorname{Im}\left(\frac{1}{A}\right)z + L),$$

so $\arg(-iL_1) \in (-\frac{\pi}{2}, \frac{\pi}{2}) \quad \forall z \geq 0$, noting

$\operatorname{Im}\left(\frac{1}{A}\right) > 0, \quad L > 0$. So just like in

the Heaviside problem we find

$$\int_0^\infty \frac{-1}{(h/A+i)} e^{i h L_1} dh = -A e^{A L_1} \left[-i\pi - E i^{\pi/2}(-A L_1) \right].$$

Similarly, we find

$$\int_{-\infty}^0 \frac{1}{(h/A+i)} e^{-z} e^{i h(x+iL)} dh = A e^{A(x+iL)} e^{-z} \\ \cdot \left(-i\pi - E i^{\pi/2}(-A(x+iL)) \right)$$

$$\int_0^\infty \frac{1}{h/A - i} e^{ihL_1} dh = A e^{-AL_1} (i\pi - \text{Ei}^\pi(AL_1))$$

$$\int_0^\infty \frac{-1}{h/A - i} e^{-z} e^{ih(x+iL)} = -A e^{-A(x+iL)} (i\pi - \text{Ei}^\pi(A(x+iL))) e^{-z}$$

$$\int_{-\infty}^0 \frac{1}{h/A + i} e^{ihL_2} dh = -A e^{AL_2} (\text{Ei}^\pi(-AL_2) + i\pi)$$

$$\int_{-\infty}^0 \frac{1}{h/A + i} e^{-z} e^{ih(x-iL)} dh = A e^{A(x-iL)} e^{-z} (\text{Ei}^\pi(-A(x-iL)) + i\pi)$$

$$\int_{-\infty}^0 \frac{1}{(h/A - i)} e^{ihL_2} dh = A e^{-AL_2} (\text{Ei}^{\pi/2}(AL_2) + i\pi)$$

$$\int_{-\infty}^0 \frac{-1}{(h/A - i)} e^{-z} e^{ih(x-iL)} = -A e^{-A(x-iL)} e^{-z} (\text{Ei}^{\pi/2}(A(x-iL)) + i\pi) e^{-z}$$

Label these integrals $I_1, I_2, \dots, I_8,$

respectively. Then

$$\psi = \text{Re} \left\{ \frac{-1}{2\pi B^2 2i} I e^{st} \right\} \quad \text{where} \quad I = \sum_{n=1}^8 I_n$$

To get u , note

$$\frac{\partial I_1}{\partial z} = I_1 - A e^{AL_1} \left(\frac{e^{-AL_1}}{-AL_1} \cdot (-1) \right) = I_1 + \frac{1}{L_1}$$

$$\frac{\partial I_2}{\partial z} = -I_2$$

$$\frac{\partial I_3}{\partial z} = -I_3 - A \frac{e^{-AL_1} e^{AL_1}}{AL_1} = -\frac{1}{L_1} - I_3$$

$$\frac{\partial I_4}{\partial z} = -I_4$$

$$\frac{\partial I_5}{\partial z} = -I_5 - A e^{AL_2} \left(\frac{e^{-AL_2}}{-AL_2} \right) \cdot 1 = -I_5 + \frac{1}{L_2}$$

$$\frac{\partial I_6}{\partial z} = -I_6$$

$$\frac{\partial I_2}{\partial z} = I_2 + A e^{-AL_2} \frac{e^{AL_2}}{AL_2} \cdot (-1) = I_2 - \frac{1}{L_2}$$

$$\frac{\partial I_8}{\partial z} = -I_8. \quad \text{So for } n \text{ we have}$$

$$u = \operatorname{Re} \left\{ \frac{-1}{2\pi \times 10^{-2} j} I_n e^{j\omega t} \right\}, \quad \text{where}$$

$$I_n = I_1 - I_2 - I_3 - I_4 - I_5 - I_6 + I_7 - I_8.$$

Similarly,

$$\frac{\partial I_1}{\partial x} = A I_1 - A e^{AL_1} \left[-\frac{e^{-AL_1}}{-AL_1} \right] \cdot (-A) = A I_1 + \frac{A}{L_1}$$

$$\begin{aligned} \frac{\partial I_2}{\partial x} &= A I_2 + A e^{A(x+jL)} e^{-z} \left(-\frac{e^{-A(x+jL)}}{-A(x+jL)} \right) \cdot (-A) \\ &= A I_2 + \frac{A(-A)e^{-z}}{A(x+jL)} = A I_2 - \frac{A e^{-z}}{(x+jL)} \end{aligned}$$

$$\frac{\partial I_3}{\partial x} = -I_3 A + A e^{-AL_1} \left(-\frac{e^{AL_1}}{AL_1} \right) \cdot A = -A I_3 - \frac{A}{L_1}$$

$$\begin{aligned} \frac{\partial I_4}{\partial x} &= -A I_4 + A e^{-A(x+jL)} \left(\frac{e^{A(x+jL)}}{A(x+jL)} \right) \cdot A e^{-z} \\ &= -A I_4 + \frac{A e^{-z}}{x+jL} \end{aligned}$$

$$\frac{\partial I_5}{\partial x} = A I_5 - A e^{AL_2} \left(\frac{e^{-AL_2}}{-AL_2} \right) \cdot (-A) = A I_5 - \frac{A}{L_2}$$

$$\begin{aligned} \frac{\partial I_6}{\partial x} &= A I_6 + A e^{A(x-jL)} e^{-z} \left(\frac{e^{-A(x-jL)}}{-A(x-jL)} \right) \cdot (-A) \\ &= A I_6 + \frac{A e^{-z}}{x-jL} \end{aligned}$$

$$\frac{\partial I_7}{\partial x} = -A I_7 + A e^{-AL_2} \left(\frac{e^{AL_2}}{AL_2} \right) \cdot A = -A I_7 + \frac{A}{L_2}$$

$$\frac{\partial I_8}{\partial x} = -A I_8 - A e^{-A(x-jL)} \left(\frac{e^{A(x-jL)}}{A(x-jL)} \right) \cdot A e^{-z} = -A I_8 - \frac{A e^{-z}}{x-jL}.$$

Now recalling $w = -\frac{\partial \psi}{\partial z}$, we have

$$w = \operatorname{Re} \left\{ \frac{-1}{2\pi B^2 z} I_w e^{it} \right\} \text{ where}$$

$$I_w = A(-I_1 - I_2 + I_3 + I_4 - I_5 - I_6 + I_7 + I_8).$$